feat(Keyring): RawRSAKeyring (#442)

aws-encryption-sdk-net-formally-verified/Examples/Keyring/RawRSAKeyring/RawRSAKeyringExample.cs
@@ -1,0 +1,108 @@
+// Copyright Amazon.com Inc. or its affiliates. All Rights Reserved.
+// SPDX-License-Identifier: Apache-2.0
+
+using System.Collections.Generic;
+using System.IO;
+
+using Aws.Crypto;
+using Aws.Esdk;
+
+using Org.BouncyCastle.Security; // In this example, we use BouncyCastle to generate a wrapping key.
+using Xunit;
+
+using ibyteseq = Dafny.ISequence<byte>;
+using byteseq = Dafny.Sequence<byte>;
+
+
+/// Demonstrate an encrypt/decrypt cycle using a raw RSA keyring.
+public class RawRSAKeyringExample {
+    static void Run(MemoryStream plaintext) {
+        // Create your encryption context.
+        // Remember that your encryption context is NOT SECRET.
+        // https://docs.aws.amazon.com/encryption-sdk/latest/developer-guide/concepts.html#encryption-context
+        Dictionary<string, string> encryptionContext = new Dictionary<string, string>() {
+            {"name", "encryption context"},
+            {"is_secret", "false"},
+            {"is_public", "true"},
+            {"purpose", "useful metadata"}
+        };
+    
+        // Generate a 2,048 bit RSA Key to use with your keyring.
+        // We generate a key with Bouncy Castle, but you could also load a key,
+        // or generate a key with another low level cryptographic library.
+        RSAEncryption.RSA.GenerateKeyPairBytes(2048, out var publicKeyBytes, out var privateKeyBytes);
+        System.IO.MemoryStream publicKey = DafnyFFI.MemoryStreamFromSequence(byteseq.FromArray(publicKeyBytes));
+        System.IO.MemoryStream privateKey = DafnyFFI.MemoryStreamFromSequence(byteseq.FromArray(privateKeyBytes));
+
+        // The key namespace and key name are defined by you
+        // and are used by the raw RSA keyring to determine
+        // whether it should attempt to decrypt an encrypted data key.
+        //
+        // https://docs.aws.amazon.com/encryption-sdk/latest/developer-guide/choose-keyring.html#use-raw-rsa-keyring
+        string keyNamespace = "Some managed raw keys";
+        string keyName = "My 2048-bit RSA wrapping key";
+
+        // Create clients to access the Encryption SDK APIs.    
+        // TODO: add client configuration objects
+        IAwsCryptographicMaterialProviders materialProviders = new AwsCryptographicMaterialProvidersClient();
+        IAwsEncryptionSdk encryptionSdkClient = new AwsEncryptionSdkClient();
+
+        // Create the keyring that determines how your data keys are protected.
+        CreateRawRsaKeyringInput createRawRsaKeyringInput = new CreateRawRsaKeyringInput
+        {
+            KeyNamespace = keyNamespace,
+            KeyName = keyName,
+            PaddingScheme = PaddingScheme.OAEP_SHA512_MGF1,
+            PublicKey = publicKey,
+            PrivateKey = privateKey
+        };
+        IKeyring keyring = materialProviders.CreateRawRsaKeyring(createRawRsaKeyringInput);
+
+        // Create the materials manager that assembles cryptographic materials from your keyring.
+        CreateDefaultCryptographicMaterialsManagerInput createMaterialsManagerInput =
+            new CreateDefaultCryptographicMaterialsManagerInput {Keyring = keyring};
+        ICryptographicMaterialsManager materialsManager =
+            materialProviders.CreateDefaultCryptographicMaterialsManager(createMaterialsManagerInput);
+
+        // Encrypt your plaintext data.
+        EncryptInput encryptInput = new EncryptInput
+        {
+            Plaintext = plaintext,
+            MaterialsManager = materialsManager,
+            EncryptionContext = encryptionContext,
+        };
+        EncryptOutput encryptOutput = encryptionSdkClient.Encrypt(encryptInput);
+        MemoryStream ciphertext = encryptOutput.Ciphertext;
+
+        // Demonstrate that the ciphertext and plaintext are different.
+        Assert.NotEqual(ciphertext.ToArray(), plaintext.ToArray());
+
+        // Decrypt your encrypted data using the same keyring you used on encrypt.
+        //
+        // You do not need to specify the encryption context on decrypt
+        // because the header of the encrypted message includes the encryption context.
+        DecryptInput decryptInput = new DecryptInput
+        {
+            Ciphertext = ciphertext,
+            MaterialsManager = materialsManager,
+        };
+        DecryptOutput decryptOutput = encryptionSdkClient.Decrypt(decryptInput);
+        MemoryStream decrypted = decryptOutput.Plaintext;
+
+        // Demonstrate that the decrypted plaintext is identical to the original plaintext.
+        Assert.Equal(decrypted.ToArray(), plaintext.ToArray());
+
+        // Verify that the encryption context used in the decrypt operation includes
+        // the encryption context that you specified when encrypting.
+        // The AWS Encryption SDK can add pairs, so don't require an exact match.
+        //
+        // In production, always use a meaningful encryption context.
+        // TODO: Add logic that checks the encryption context.        
+    }
+
+    // We test examples to ensure they remain up-to-date.
+    [Fact]
+    public void TestRawRSAKeyringExample() {
+        Run(ExampleUtils.ExampleUtils.GetPlaintextStream());
+    }
+}
